WIP ooo_input_op

dataplane/Examples/Ooo_Input_op.thy
@@ -7,13 +7,108 @@ begin
 
 record ('p, 'd, 'd1, 't) input_state = "('p, 'd, 'd1, 't) operator_state_ty" + es:: "'p \<Rightarrow> ('t, 'd1) event llist"
 
+abbreviation \<open>ooo_input_op_logic ops os \<equiv> cimage (\<lambda>p. case es os p of
+    LNil \<Rightarrow> drop_caps os (map (\<lambda>t. Cap t p) (ocaps os p))
+  | LCons (Data t d) lxs \<Rightarrow> produce (os\<lparr>es := (es os)(p := lxs)\<rparr>) (Cap t p) [en1 os d]
+  | LCons (Drop t) lxs \<Rightarrow> drop_cap (os\<lparr>es := (es os)(p := lxs)\<rparr>) (Cap t p)
+  | LCons (Mint t) lxs \<Rightarrow> add_cap (os\<lparr>es := (es os)(p := lxs)\<rparr>) p t)
+    (cfilter (\<lambda>p. ocaps os p \<noteq> []) ops)\<close>
+
 definition ooo_input_op where
-  "ooo_input_op ops os = builder_op {||} ops os (\<lambda> os. (cimage (\<lambda>p. case es os p of
-    LNil \<Rightarrow> drop_caps os (map (\<lambda> t. Cap t p) (ocaps os p))
-  | LCons (Data t d) lxs \<Rightarrow> produce (os\<lparr> es := (es os)(p := lxs) \<rparr>) (Cap t p) [en1 os d]
-  | LCons (Drop t) lxs \<Rightarrow> drop_cap (os\<lparr> es := (es os)(p := lxs) \<rparr>) (Cap t p)
-  | LCons (Mint t) lxs \<Rightarrow> mint_cap (os\<lparr> es := (es os)(p := lxs) \<rparr>) p t)
-    (cfilter (\<lambda>p. ocaps os p \<noteq> []) ops)))"
+  "ooo_input_op ops os = builder_op {||} ops os (ooo_input_op_logic ops)"
+
+abbreviation ooo_inp_op where
+  \<open>ooo_inp_op ops os \<equiv>
+  map_op (case_option (Inl (0 :: 1)) (\<lambda>p. Inr (0 :: 1, p))) (case_option (Inl (0 :: 1)) (\<lambda>p. Inr (0 :: 1, p)))
+  (ooo_input_op ops os)\<close>
+
+abbreviation ooo_inp_summary where
+  \<open>ooo_inp_summary \<equiv> (\<lambda>l1 l2.
+  if l1 = Loc (0 :: 1) (Trg (0 :: 1)) \<and> l2 = Loc (0 :: 1) (Src (0 :: 1))
+  then antichain {0}
+  else {}\<^sub>A)\<close>
+
+abbreviation ooo_input_os_Drop_Mint where
+  \<open>ooo_input_os_Drop_Mint p os e \<equiv> (case e of
+    Drop t \<Rightarrow> drop_cap os (Cap t p)
+  | Mint t \<Rightarrow> add_cap os p t)\<close>
+
+lemma initia_foldl_ooo_input_os_Drop_Mint:
+  \<open>initia os \<Longrightarrow> \<forall>e \<in> set xs. \<not> is_Data e \<Longrightarrow> initia (foldl (ooo_input_os_Drop_Mint p) os xs)\<close>
+  by (induction xs arbitrary: os) (auto split: event.splits)
+
+lemma outpu_foldl_ooo_input_os_Drop_Mint:
+  \<open>outpu os p = [] \<Longrightarrow> \<forall>e \<in> set xs. \<not> is_Data e \<Longrightarrow> outpu (foldl (ooo_input_os_Drop_Mint p) os xs) p = []\<close>
+  by (induction xs arbitrary: os) (auto split: event.splits)
+
+lemma en1_foldl_ooo_input_os_Drop_Mint:
+  \<open>\<forall>e \<in> set xs. \<not> is_Data e \<Longrightarrow> en1 os = en1 (foldl (ooo_input_os_Drop_Mint p) os xs)\<close>
+  by (induction xs arbitrary: os) (auto split: event.splits)
+
+(* TODO prove and move *)
+lemma mset_remove_last:
+  \<open>mset (remove_last x xs) = mset xs - {#x#}\<close>
+  apply (induction x xs rule: remove_last.induct)
+  sorry
+
+lemma step_Taus_ooo_input_op_Drop_Mint:
+  \<open>lfinite (ltakeWhile (Not \<circ> is_Data) (es os p)) \<Longrightarrow>
+  ldropWhile (Not \<circ> is_Data) (es os p) = LCons (Data t d) lxs \<Longrightarrow> p |\<in>| ops \<Longrightarrow>
+  op = ooo_input_op ops os \<Longrightarrow> initia os \<Longrightarrow> monotone (es os p) (mset (ocaps os p)) \<Longrightarrow>
+  os' = foldl (ooo_input_os_Drop_Mint p) os (list_of (ltakeWhile (Not \<circ> is_Data) (es os p))) \<Longrightarrow>
+  os'' = produce (os'\<lparr>es := (es os')(p := lxs)\<rparr>) (Cap t p) [en1 os' d] \<Longrightarrow> op' = ooo_input_op ops os'' \<Longrightarrow>
+  (step Tau)\<^sup>*\<^sup>* op op'\<close>
+  unfolding ooo_input_op_def
+proof (induction \<open>ltakeWhile (Not \<circ> is_Data) (es os p)\<close> arbitrary: os op rule: lfinite_induct)
+  case LNil
+  have \<open>ldropWhile (Not \<circ> is_Data) (es os p) = es os p\<close>
+    using LNil(1) ldropWhile_LCons ldropWhile_LNil llist.sel(1) lnull_def ltakeWhile_eq_LNil_iff neq_LNil_conv
+    by metis
+  moreover from this have \<open>ocaps os p \<noteq> []\<close>
+    using LNil(2,6) monotone.cases by force
+  ultimately have \<open>os'' |\<in>| ooo_input_op_logic ops os\<close>
+    using LNil(2,3,7,8) by force
+  thus ?case
+    using LNil(4,5,9) step_builder_op_Silent ooo_input_op_def by blast
+next
+  case LCons
+  obtain e where head_es: \<open>\<not> is_Data e\<close> \<open>lhd (es os p) = e\<close> \<open>es os p = LCons e (ltl (es os p))\<close>
+    using LCons(2) by fastforce
+  let ?os1 = \<open>ooo_input_os_Drop_Mint p (os\<lparr>es := (es os)(p := ltl (es os p))\<rparr>) e\<close>
+  have ocaps_not_empty: \<open>ocaps os p \<noteq> []\<close>
+    using LCons(8) head_es(3) monotone.cases by force
+  hence \<open>?os1 |\<in>| ooo_input_op_logic ops os\<close>
+    using LCons(5) head_es(1,3) cin_cimage_cfilter event.case_eq_if input_state.fold_congs(12)
+      llist.case(2) operator_state.unfold_congs(3,8) by (smt (verit))
+  hence \<open>step Tau op (ooo_input_op ops ?os1)\<close>
+    using LCons(6,7) step_builder_op_Silent[of os] ooo_input_op_def by blast
+  moreover have \<open>(step Tau)\<^sup>*\<^sup>* (ooo_input_op ops ?os1) op'\<close>
+  proof -
+    have es_os1: \<open>es ?os1 p = ltl (es os p)\<close>
+      using head_es(1) by (auto split: event.splits)
+    hence \<open>ltl (ltakeWhile (Not \<circ> is_Data) (es os p)) = ltakeWhile (Not \<circ> is_Data) (es ?os1 p)\<close>
+      using LCons(2) lnull_ltakeWhile ltakeWhile.simps(4) by force
+    moreover from this have \<open>ldropWhile (Not \<circ> is_Data) (es ?os1 p) = LCons (Data t d) lxs\<close>
+      using LCons(2,4) es_os1 ldropWhile_simps(2) lhd_LCons_ltl ltakeWhile.disc(1) by metis
+    moreover have \<open>initia ?os1\<close>
+      using LCons(7) head_es(1) by (auto split: event.splits)
+    moreover have \<open>monotone (es ?os1 p) (mset (ocaps ?os1 p))\<close>
+      using LCons(8) ocaps_not_empty head_es es_os1 monotone.cases
+      apply (auto split: event.splits)
+      using mset_remove_last event.distinct(1,6) event.inject(2) llist.inject monotone.cases mset_zero_iff
+       apply (smt (verit))
+      apply fastforce
+      done
+    moreover have \<open>os' = foldl (ooo_input_os_Drop_Mint p) ?os1 (list_of (ltakeWhile (Not \<circ> is_Data) (es ?os1 p)))\<close>
+      using LCons(9) es_os1
+      (* TODO Fix the hypothesis on os'. *)
+      sorry
+    ultimately show ?thesis
+      using LCons(3,5,10,11) ooo_input_op_def by blast
+  qed
+  ultimately show ?case
+    by (rule transitive_closurep_trans'(6))
+  oops
 
 record ('p, 'd, 'd1, 'd2, 't) input_state2 = "('p, 'd, 'd1, 'd2, 't) operator_state_ty2" + 
   es1:: "('t, 'd1) event llist" es2:: "('t, 'd2) event llist"
